Added examples for the new sp and while

examples/sp_free.ec
@@ -10,22 +10,30 @@ module MAIN = {
     }
     return i;
   }
+  proc id_call (n : int) : int = {
+    var i;
+    i <- id_while(n);
+    return i;
+  }
+  (*TODO: is this the bad case?*)
+  proc id_if (n : int) : int = {
+    var i;
+    i <- 0;
+    if (n <> 0) {
+      i <- n;
+    }
+    return i;
+  }
 }.
 
 lemma id_while_free m :
-  hoare [MAIN.nth_odd : m = 0 ==> m = 0].
-proof.
-  proc; sp.
-  while ((0 <= i <= n) /\ (x = 2 * i + 1)).
-  + by auto => /> /#.
-  by auto => /> /#.
-qed.
+  hoare [MAIN.id_while : m = 0 ==> m = 0].
+proof. by proc; sp; skip. qed.
 
-lemma nth_odd_spec_for m :
-  hoare [MAIN.nth_odd : (n = m) /\ (0 <= n) ==> res = (2 * m + 1)].
-proof.
-  proc.
-  for (fun i => (x = 2 * i + 1)) => /=.
-  + by auto => /> /#.
-  by auto => /> /#.
-qed.
+lemma id_call_free m :
+  hoare [MAIN.id_call : m = 0 ==> m = 0].
+proof. by proc; sp; skip. qed.
+
+lemma id_if_free m :
+  hoare [MAIN.id_if : m = 0 ==> m = 0].
+proof. by proc; sp; skip. qed.
