examples/while_free.ec
@@ -1,0 +1,23 @@
+require import AllCore Int StdOrder.
+import IntOrder.
+
+module MAIN = {
+  proc id_while (n : int) : int = {
+    var i, one;
+    i <- 0;
+    one <- 1;
+    while (i < n) {
+      i <- i + one;
+    }
+    return i;
+  }
+}.
+
+lemma double_while_double m :
+  hoare [MAIN.id_while : (m = n) /\ (0 <= n) ==> res = m].
+proof.
+  proc; sp.
+  while(i <= n).
+  + by sp; skip => /> /#.
+  by skip => /> /#.
+qed.
